src/program_proof/leasekv/proof.v
@@ -1,35 +1,267 @@
 From Perennial.program_proof Require Import grove_prelude.
 From Perennial.program_logic Require Import atomic.
 From Goose.github_com.mit_pdos.gokv Require Import leasekv.
-From iris.base_logic.lib Require Import ghost_map.
+From Perennial.program_proof.simplepb Require Import renewable_lease.
+From Perennial.program_proof.fencing Require Import map.
+
+Module cacheValueC.
+Record t :=
+  mk {
+      v : string ;
+      l : u64 ;
+    }.
+
+#[global] Instance into_val : IntoVal t.
+Proof.
+  refine {| into_val.to_val := (λ (x:t),
+                                 struct.mk_f cacheValue [
+                                     "v" ::= #(LitString x.(v)) ;
+                                     "l" ::= #x.(l)
+                                   ])%V ;
+           from_val := λ v, match v with (#(LitString v), (#(LitInt t), #()))%V => Some (mk v t) | _ => None end ;
+           IntoVal_def := mk "" (U64 0) ;
+         |}.
+  intros. simpl. by destruct v0.
+Defined.
+
+#[global] Instance into_val_for_type : IntoValForType t (struct.t cacheValue).
+Proof. constructor; auto. Qed.
+
+End cacheValueC.
 
 Section proof.
 Context `{!heapGS Σ}.
-Context `{!ghost_mapG Σ string string}.
+Context `{!mapG Σ string string}.
+Context `{!renewable_leaseG Σ}.
+Context {kvptsto: string → string → iProp Σ}.
 
 (* Specification of Kv interface. *)
-Definition is_Kv_Put Put_fn γ : iProp Σ :=
+Definition is_Kv_Put (Put_fn:val) : iProp Σ :=
   ∀ key value,
   {{{ True }}}
-  <<< ∀∀ old_value, key ↪[γ] old_value >>>
+  <<< ∀∀ old_value, kvptsto key old_value >>>
     Put_fn #(LitString key) #(LitString value) @ ∅
-  <<< key ↪[γ] value >>>
+  <<< kvptsto key value >>>
   {{{ RET #(); True }}}.
 
-Definition is_Kv_Get Get_fn γ : iProp Σ :=
+Definition is_Kv_Get (Get_fn:val) : iProp Σ :=
   ∀ key,
   {{{ True }}}
-  <<< ∀∀ value, key ↪[γ] value >>>
+  <<< ∀∀ value, kvptsto key value >>>
     Get_fn #(LitString key) @ ∅
-  <<< key ↪[γ] value >>>
+  <<< kvptsto key value >>>
   {{{ RET #(LitString value); True }}}.
 
-Definition is_Kv_ConditionalPut CondPut_fn γ : iProp Σ :=
+Definition is_Kv_ConditionalPut (CondPut_fn:val) : iProp Σ :=
   ∀ key expect value,
   {{{ True }}}
-  <<< ∀∀ old_value, key ↪[γ] old_value >>>
+  <<< ∀∀ old_value, kvptsto key old_value >>>
     CondPut_fn #(LitString key) #(LitString expect) #(LitString value) @ ∅
-  <<< key ↪[γ] (if bool_decide (expect = old_value) then value else old_value) >>>
+  <<< kvptsto key (if bool_decide (expect = old_value) then value else old_value) >>>
   {{{ RET #(LitString (if bool_decide (expect = old_value) then "ok" else "")); True }}}.
+
+Definition is_Kv (k:loc) : iProp Σ :=
+  ∃ Put_fn Get_fn CondPut_fn,
+  "#Hput" ∷ readonly (k ↦[Kv :: "Put"] Put_fn) ∗
+  "#HputSpec" ∷ is_Kv_Put Put_fn ∗
+
+  "#Hget" ∷ readonly (k ↦[Kv :: "Get"] Get_fn) ∗
+  "#HgetSpec" ∷ is_Kv_Get Get_fn ∗
+
+  "#Hcput" ∷ readonly (k ↦[Kv :: "ConditionalPut"] CondPut_fn) ∗
+  "#HcputSpec" ∷ is_Kv_ConditionalPut CondPut_fn
+.
+
+(* FIXME: copies from tutorial proof *)
+Fixpoint string_le (s:string): list u8 :=
+  match s with
+  | EmptyString => []
+  | String x srest => [U8 (Ascii.nat_of_ascii x)] ++ (string_le srest)
+  end
+.
+
+Definition encode_cacheValue (v:string) (lease:u64) : string.
+Admitted.
+
+Definition leaseN := nroot .@ "lease".
+Definition invN := nroot .@ "lease".
+
+Definition is_inv γ : iProp Σ :=
+  inv invN (∃ kvs leases,
+    "Hmap" ∷ ([∗ map] k ↦ v; lease ∈ kvs ; leases,
+                             kvptsto k (encode_cacheValue v lease) ∗
+                             ((∃ γl, own_lease_expiration γl lease ∗
+                                    is_lease leaseN γl (k ⤳[γ]{#1/2} v) ∗
+                                    post_lease leaseN γl (k ⤳[γ]{#1/2} v)) ∨
+                             (k ⤳[γ]{#1/2} v)))
+           )
+.
+
+Definition own_LeaseKv (k:loc) (γ:gname) : iProp Σ :=
+  ∃ (cache_ptr:loc) (cache:gmap string cacheValueC.t),
+  "Hcache_ptr" ∷ k ↦[LeaseKv :: "cache"] #cache_ptr ∗
+  "Hcache" ∷ own_map cache_ptr 1 cache ∗
+  "#Hleases" ∷ ([∗ map] k ↦ cv ∈ cache,
+                  ∃ γl, is_lease leaseN γl (k ⤳[γ]{#1/2} cv.(cacheValueC.v)) ∗
+                        is_lease_valid_lb γl cv.(cacheValueC.l)
+               )
+.
+
+Definition is_LeaseKv (k:loc) γ : iProp Σ :=
+  ∃ mu (kv:loc),
+  "#Hinv" ∷ is_inv γ ∗
+  "#Hmu" ∷ readonly (k ↦[LeaseKv :: "mu"] mu) ∗
+  "#HmuInv" ∷ is_lock nroot mu (own_LeaseKv k γ) ∗
+  "#Hkv" ∷ readonly (k ↦[LeaseKv :: "kv"] #kv) ∗
+  "#Hkv_is" ∷ is_Kv kv
+.
+
+Lemma wp_DecodeValue v l :
+  {{{ True }}}
+  DecodeValue #(str encode_cacheValue v l)
+  {{{ RET (to_val (cacheValueC.mk v l)); True }}}.
+Proof.
+Admitted.
+
+Lemma wp_LeaseKv__Get (k:loc) key γ :
+  ⊢ {{{ is_LeaseKv k γ }}}
+    <<< ∀∀ v, key ⤳[γ]{#1/2} v >>>
+      LeaseKv__Get #k #(LitString key) @ ↑leaseN ∪ ↑invN
+    <<< key ⤳[γ]{#1/2} v >>>
+  {{{ RET #(LitString v); True }}}.
+Proof.
+  Opaque struct.get.
+  iIntros (?) "!# Hkv Hau".
+  wp_lam.
+  wp_pures.
+  iNamed "Hkv".
+  wp_loadField.
+  wp_apply (acquire_spec with "[$]").
+  iIntros "[Hlocked Hown]".
+  iNamed "Hown".
+  wp_pures.
+  wp_loadField.
+  wp_apply (wp_MapGet with "[$]").
+  iIntros (??) "[%Hlookup Hcache]".
+  wp_pures.
+  wp_apply wp_GetTimeRange.
+  iIntros "* %Hh %Hl Htime".
+  destruct (decide (ok = true ∧ int.nat h < int.nat v.(cacheValueC.l))) as [Hvalid|Hnot].
+  {
+    (* case: cache is valid *)
+    destruct Hvalid as [? Hvalid]. subst.
+    apply map_get_true in Hlookup.
+    iDestruct (big_sepM_lookup_acc with "Hleases") as "[#H _]".
+    { done. }
+    iDestruct "H" as (?) "[#Hlease #Hvalid]".
+    iMod (lease_acc with "[$] [$] [$]") as "[>Hkey Hclose]".
+    { done. }
+    { word. }
+    iMod ncfupd_mask_subseteq as "Hmask".
+    2: iMod "Hau" as (?) "[Hkey2 Hau]".
+    { solve_ndisj. }
+    iDestruct (ghost_map_points_to_agree with "[$] [$]") as %?.
+    subst.
+    iMod ("Hau" with "[$]") as "HΦ".
+    iMod "Hmask" as "_".
+    iMod ("Hclose" with "[$]") as "Htime".
+    iModIntro.
+    iFrame.
+    wp_pures.
+    Transparent struct.get. wp_pures.
+    wp_if_destruct.
+    2:{ exfalso. word. }
+    wp_loadField.
+    wp_apply (release_spec with "[-HΦ]").
+    { iFrame "HmuInv∗". iNext.
+      repeat iExists _; eauto with iFrame.
+    }
+    wp_pures.
+    by iApply "HΦ".
+  }
+  { (* case: cache is not valid, have to actually call Kv.Get() *)
+    iFrame. iModIntro.
+    wp_pures.
+    wp_apply (wp_and).
+    { iAccu. }
+    { wp_pures. iPureIntro. instantiate (2:=(ok = true)). destruct ok.
+      * by rewrite bool_decide_true.
+      * by rewrite bool_decide_false.
+    }
+    { iIntros. Transparent struct.get. wp_pures. done. }
+    iIntros "_".
+    rewrite bool_decide_false.
+    2:{ intros [H H2]. subst. apply Hnot. split; first done. word. }
+    wp_pures.
+    wp_loadField.
+    wp_apply (wp_MapDelete with "[$]").
+    iIntros "Hcache".
+    wp_pures.
+    wp_loadField.
+    wp_apply (release_spec with "[-Hau]").
+    { iFrame "HmuInv∗". iNext.
+      repeat iExists _.
+      iFrame.
+      iApply (big_sepM_subseteq with "Hleases").
+      unfold map_del.
+      apply delete_subseteq.
+    }
+    wp_pure1_credit "Hlc".
+    wp_loadField.
+    iNamed "Hkv_is".
+    wp_loadField.
+    wp_apply ("HgetSpec" with "[//]").
+    iInv "Hinv" as "Hi" "Hclose".
+    iMod (lc_fupd_elim_later with "Hlc Hi") as "Hi".
+    iNamed "Hi".
+    iMod ncfupd_mask_subseteq as "Hmask".
+    2: iMod "Hau".
+    { solve_ndisj. }
+    iModIntro.
+    iDestruct "Hau" as (?) "[Hkey Hau]".
+    clear Hlookup.
+    assert (∃ v, kvs !! key = Some v) as [? Hlookup].
+    { admit. } (* FIXME: deal with infinite map domain *)
+    iDestruct (big_sepM2_lookup_l_some with "Hmap") as %[? HleaseLookup].
+    { done. }
+    iDestruct (big_sepM2_lookup_acc with "Hmap") as "[HH Hmap]".
+    1-2: done.
+    iDestruct "HH" as "[Hkvptsto Hrest]".
+    iAssert (⌜v0 = x⌝)%I with "[-]" as %?.
+    {
+      (* TODO: match up x in Hrest with v 0 from Hkey; naively, this requires
+         destructing into two cases: either the lease is expired, or it isn't.
+         This same annoyance showed up in the simplepb config service proof.
+         Ideally, we shouldn't need to do destruct, and should be able to make
+         use of the fact that---one way or another---we have access to `key ⤳ x`,
+         and that's all we need.
+         This will also require adjusting some masks, so we have access to the
+         lease resource here.
+       *)
+      (* XXX: Here's a hacky solution:
+         "Hrest" always directly maintains 1/4 ownership, and the other 1/4
+         might be in a lease.
+      *)
+      admit.
+    }
+    subst.
+    iExists _.
+    iFrame.
+    iIntros "Hkvptsto".
+    iSpecialize ("Hmap" with "[$]").
+    iMod ("Hau" with "[$]") as "HΦ".
+    iMod "Hmask".
+    iMod ("Hclose" with "[Hmap]") as "_".
+    { iNext. repeat iExists _; iFrame. }
+    iModIntro.
+    iIntros "_".
+    wp_pures.
+    wp_apply wp_DecodeValue.
+    wp_pures.
+    iModIntro. by iApply "HΦ".
+  }
+  Unshelve.
+  apply _.
+Admitted.
 
 End proof.
